Valaig/Utils/GrindIter.lean
@@ -1,0 +1,366 @@
+module
+
+public import Std.Data.Iterators.Lemmas
+
+public section
+
+/-
+This module just marks some useful iterator based simp lemmas as grind, making them more useful.
+-/
+
+-- Init.Data.Iterators.Lemmas.Combinators.Monadic.FilterMap
+attribute [simp, grind =]
+  Std.IterM.toList_filterMap
+  Std.IterM.toList_mapM
+  Std.IterM.toList_map
+  Std.IterM.toList_filter
+  Std.IterM.toListRev_filterMap
+  Std.IterM.toListRev_map
+  Std.IterM.toListRev_filter
+  Std.IterM.toArray_filterMap
+  Std.IterM.toArray_mapM
+  Std.IterM.toArray_map
+  Std.IterM.toArray_filter
+  Std.IterM.forIn_filterMapM
+  Std.IterM.forIn_filterMap
+  Std.IterM.forIn_mapM
+  Std.IterM.forIn_map
+  Std.IterM.forIn_filterM
+  Std.IterM.forIn_filter
+  Std.IterM.foldM_filterMapM
+  Std.IterM.foldM_mapM
+  Std.IterM.foldM_filterM
+  Std.IterM.foldM_filterMap
+  Std.IterM.foldM_map
+  Std.IterM.foldM_filter
+  Std.IterM.fold_filterMapM
+  Std.IterM.fold_mapM
+  Std.IterM.fold_filterM
+  Std.IterM.fold_filterMap
+  Std.IterM.fold_map
+  Std.IterM.fold_filter
+  Std.IterM.length_map
+  Std.IterM.anyM_filterMap
+  Std.IterM.anyM_map
+  Std.IterM.anyM_filter
+  Std.IterM.any_filterMap
+  Std.IterM.any_map
+  Std.IterM.allM_filterMap
+  Std.IterM.allM_map
+  Std.IterM.allM_filter
+  Std.IterM.all_filterMap
+  Std.IterM.all_map
+
+-- Init.Data.Iterators.Lemmas.Combinators.Monadic.FlatMap
+attribute [simp, grind =]
+  Std.IterM.toList_flatMapAfterM
+  Std.IterM.toArray_flatMapAfterM
+  Std.IterM.toList_flatMapM
+  Std.IterM.toArray_flatMapM
+  Std.IterM.toList_flatMapAfter
+  Std.IterM.toArray_flatMapAfter
+  Std.IterM.toList_flatMap
+  Std.IterM.toArray_flatMap
+
+-- Init.Data.Iterators.Lemmas.Combinators.Monadic.Take
+attribute [simp, grind =]
+  Std.IterM.toList_take_zero
+  Std.IterM.toList_toTake
+
+-- Init.Data.Iterators.Lemmas.Combinators.FilterMap
+attribute [simp, grind =]
+  Std.Iter.toList_filterMap
+  Std.Iter.toList_mapM
+  Std.Iter.toList_map
+  Std.Iter.toList_filter
+  Std.Iter.toListRev_filterMap
+  Std.Iter.toListRev_map
+  Std.Iter.toListRev_filter
+  Std.Iter.toArray_filterMap
+  Std.Iter.toArray_mapM
+  Std.Iter.toArray_map
+  Std.Iter.toArray_filter
+  Std.Iter.forIn_filterMapM
+  Std.Iter.forIn_filterMap
+  Std.Iter.forIn_mapM
+  Std.Iter.forIn_map
+  Std.Iter.forIn_filterM
+  Std.Iter.forIn_filter
+  Std.Iter.foldM_filterMapM
+  Std.Iter.foldM_mapM
+  Std.Iter.foldM_filterM
+  Std.Iter.foldM_filterMap
+  Std.Iter.foldM_map
+  Std.Iter.foldM_filter
+  Std.Iter.fold_filterMapM
+  Std.Iter.fold_mapM
+  Std.Iter.fold_filterM
+  Std.Iter.fold_filterMap
+  Std.Iter.fold_map
+  Std.Iter.fold_filter
+  Std.Iter.length_map
+  Std.Iter.anyM_filterMap
+  Std.Iter.anyM_map
+  Std.Iter.anyM_filter
+  Std.Iter.any_filterMap
+  Std.Iter.any_map
+  Std.Iter.allM_filterMap
+  Std.Iter.allM_map
+  Std.Iter.allM_filter
+  Std.Iter.all_mapM
+  Std.Iter.all_filterMap
+  Std.Iter.all_map
+
+-- Init.Data.Iterators.Lemmas.Combinators.FlatMap
+attribute [simp, grind =]
+  Std.Iter.toList_flatMapAfterM
+  Std.Iter.toArray_flatMapAfterM
+  Std.Iter.toList_flatMapM
+  Std.Iter.toArray_flatMapM
+  Std.Iter.toList_flatMapAfter
+  Std.Iter.toArray_flatMapAfter
+  Std.Iter.toList_flatMap
+  Std.Iter.toArray_flatMap
+
+-- Init.Data.Iterators.Lemmas.Combinators.Take
+attribute [simp, grind =]
+  Std.Iter.toList_take_of_finite
+  Std.Iter.toListRev_take_of_finite
+  Std.Iter.toArray_take_of_finite
+  Std.Iter.toList_take_zero
+  Std.Iter.toList_toTake
+
+-- Init.Data.Iterators.Lemmas.Consumers.Combinators.Collect
+attribute [simp, grind =]
+  Std.IterM.toArray_ensureTermination
+  Std.IterM.toList_ensureTermination
+  Std.IterM.toListRev_ensureTermination_eq_toListRev
+  Std.IterM.toList_toArray
+  Std.IterM.toList_toArray_ensureTermination
+  Std.IterM.toArray_toList
+  Std.IterM.toArray_toList_ensureTermination
+  Std.IterM.reverse_toListRev
+  Std.IterM.reverse_toListRev_ensureTermination
+  Std.IterM.toListRev_eq
+  Std.IterM.toListRev_ensureTermination
+
+-- Init.Data.Iterators.Lemmas.Consumers.Collect
+attribute [simp, grind =]
+  Std.Iter.toArray_ensureTermination
+  Std.Iter.toList_ensureTermination
+  Std.Iter.toListRev_ensureTermination_eq_toListRev
+  Std.Iter.toList_toArray
+  Std.Iter.toList_toArray_ensureTermination
+  Std.Iter.toArray_toList
+  Std.Iter.toArray_toList_ensureTermination
+  Std.Iter.reverse_toListRev
+  Std.Iter.reverse_toListRev_ensureTermination
+  Std.Iter.toListRev_eq
+  Std.Iter.toListRev_ensureTermination
+
+-- Init.Data.Iterators.Lemmas.Consumers.Loop
+attribute [simp, grind =]
+  Std.Iter.size_toArray_eq_length
+  Std.Iter.length_toList_eq_length
+  Std.Iter.length_toListRev_eq_length
+
+-- Init.Data.Iterators.Lemmas.Producers.Monadic.List
+attribute [simp, grind =]
+  List.step_iterM_nil
+  List.step_iterM_cons
+  List.step_iterM
+  List.toArray_iterM
+  List.toList_iterM
+  List.toListRev_iterM
+
+-- Init.Data.Iterators.Lemmas.Producers.List
+attribute [simp, grind =]
+  List.step_iter_nil
+  List.step_iter_cons
+  List.toArray_iter
+  List.toList_iter
+  List.toListRev_iter
+
+-- Std.Data.Iterators.Lemmas.Combinators.Drop
+attribute [simp, grind =]
+  Std.Iter.toList_drop
+  Std.Iter.toListRev_drop
+  Std.Iter.toArray_drop
+
+-- Std.Data.Iterators.Lemmas.Combinators.DropWhile
+attribute [simp, grind =]
+  Std.Iter.toList_dropWhile_of_finite
+  Std.Iter.toArray_dropWhile_of_finite
+  Std.Iter.toListRev_dropWhile_of_finite
+
+-- Std.Data.Iterators.Lemmas.Combinators.TakeWhile
+attribute [simp, grind =]
+  Std.Iter.toList_takeWhile_of_finite
+  Std.Iter.toListRev_takeWhile_of_finite
+  Std.Iter.toArray_takeWhile_of_finite
+
+-- Std.Data.Iterators.Lemmas.Combinators.Zip
+attribute [simp, grind =]
+  Std.Iter.toList_zip_of_finite
+  Std.Iter.toListRev_zip_of_finite
+  Std.Iter.toArray_zip_of_finite
+  Std.Iter.toList_take_zip
+  Std.Iter.toListRev_take_zip
+  Std.Iter.toArray_take_zip
+
+-- Std.Data.Iterators.Lemmas.Consumers.Monadic.Collect
+attribute [simp, grind =>]
+  Std.IterM.Equiv.toListRev_eq
+  Std.IterM.Equiv.toList_eq
+  Std.IterM.Equiv.toArray_eq
+
+-- Std.Data.Iterators.Lemmas.Consumers.Monadic.Loop
+attribute [simp, grind =>]
+  Std.IterM.Equiv.forIn_eq
+  Std.IterM.Equiv.foldM_eq
+  Std.IterM.Equiv.fold_eq
+  Std.IterM.Equiv.drain_eq
+
+-- Std.Data.Iterators.Lemmas.Consumers.Monadic.Loop
+attribute [simp, grind =]
+  Std.IterM.toHashSet_eq_fold
+  Std.IterM.toExtHashSet_eq_ofList
+  Std.IterM.toTreeSet_eq_fold
+  Std.IterM.toExtTreeSet_eq_ofList
+
+-- Std.Data.Iterators.Lemmas.Consumers.Collect
+attribute [simp, grind =>]
+  Std.Iter.Equiv.toListRev_eq
+  Std.Iter.Equiv.toList_eq
+  Std.Iter.Equiv.toArray_eq
+
+-- Std.Data.Iterators.Lemmas.Consumers.Loop
+attribute [simp, grind =>]
+  Std.Iter.Equiv.forIn_eq
+  Std.Iter.Equiv.foldM_eq
+  Std.Iter.Equiv.fold_eq
+
+-- Std.Data.Iterators.Lemmas.Consumers.Set
+attribute [simp, grind =]
+  Std.Iter.toExtHashSet_eq_ofList
+  Std.Iter.toExtTreeSet_eq_ofList
+attribute [grind! .]
+  Std.Iter.toHashSet_equiv_ofList
+  Std.Iter.toTreeSet_equiv_ofList
+
+-- Std.Data.Iterators.Lemmas.Producers.Monadic.Array
+attribute [simp, grind =]
+  Array.toList_iterFromIdxM
+  Array.toList_iterM
+  Array.toArray_iterFromIdxM
+  Array.toArray_iterM
+  Array.toListRev_iterFromIdxM
+  Array.toListRev_iterM
+  Array.length_iterFromIdxM
+  Array.length_iterM
+
+-- Std.Data.Iterators.Lemmas.Producers.Monadic.Empty
+attribute [simp, grind =]
+  Std.IterM.step_empty
+  Std.IterM.toList_empty
+  Std.IterM.toListRev_empty
+  Std.IterM.toArray_empty
+  Std.IterM.forIn_empty
+  Std.IterM.foldM_empty
+  Std.IterM.fold_empty
+  Std.IterM.drain_empty
+
+-- Std.Data.Iterators.Lemmas.Producers.Monadic.Vector
+attribute [simp, grind =]
+  Vector.iterFromIdxM_toArray
+  Vector.iterM_toArray
+  Vector.toList_iterFromIdxM
+  Vector.toList_iterM
+  Vector.toArray_iterFromIdxM
+  Vector.toArray_iterM
+  Vector.toListRev_iterFromIdxM
+  Vector.toListRev_iterM
+  Vector.length_iterFromIdxM
+  Vector.length_iterM
+
+-- Std.Data.Iterators.Lemmas.Producers.Array
+attribute [simp, grind =]
+  Array.toList_iterFromIdx
+  Array.toList_iter
+  Array.toArray_iterFromIdx
+  Array.toArray_iter
+  Array.toListRev_iterFromIdx
+  Array.toListRev_iter
+  Array.length_iterFromIdx
+  Array.length_iter
+
+-- Std.Data.Iterators.Lemmas.Producers.Empty
+attribute [simp, grind =]
+  Std.Iter.toIterM_empty
+  Std.Iter.step_empty
+  Std.Iter.toList_empty
+  Std.Iter.toListRev_empty
+  Std.Iter.toArray_empty
+  Std.Iter.forIn_empty
+  Std.Iter.foldM_empty
+  Std.Iter.fold_empty
+
+-- Std.Data.Iterators.Lemmas.Producers.Range
+attribute [simp, grind =]
+  Std.Rcc.toList_iter
+  Std.Rcc.toArray_iter
+  Std.Rcc.length_iter
+  Std.Rco.toList_iter
+  Std.Rco.toArray_iter
+  Std.Rco.length_iter
+  Std.Rci.toList_iter
+  Std.Rci.toArray_iter
+  Std.Rci.length_iter
+  Std.Roc.toList_iter
+  Std.Roc.toArray_iter
+  Std.Roc.length_iter
+  Std.Roo.toList_iter
+  Std.Roo.toArray_iter
+  Std.Roo.length_iter
+  Std.Roi.toList_iter
+  Std.Roi.toArray_iter
+  Std.Roi.length_iter
+  Std.Ric.toList_iter
+  Std.Ric.toArray_iter
+  Std.Ric.length_iter
+  Std.Rio.toList_iter
+  Std.Rio.toArray_iter
+  Std.Rio.length_iter
+  Std.Rii.toList_iter
+  Std.Rii.toArray_iter
+  Std.Rii.length_iter
+
+-- Std.Data.Iterators.Lemmas.Producers.Repeat
+attribute [simp, grind =]
+  Std.Iter.atIdxSlow?_repeat
+  Std.Iter.toList_take_repeat_succ
+
+-- Std.Data.Iterators.Lemmas.Producers.Slice
+attribute [simp, grind =]
+  Std.Slice.forIn_iter
+  Std.Slice.foldlM_iter
+  Std.Slice.foldl_iter
+  Std.Slice.length_iter_eq_size
+  Std.Slice.toArray_iter
+  Std.Slice.toList_iter
+  Std.Slice.toListRev_iter
+  Std.Slice.fold_iter
+  Std.Slice.foldM_iter
+
+-- Std.Data.Iterators.Lemmas.Producers.Vector
+attribute [simp, grind =]
+  Vector.iterFromIdx_toArray
+  Vector.iter_toArray
+  Vector.toList_iterFromIdx
+  Vector.toList_iter
+  Vector.toArray_iterFromIdx
+  Vector.toArray_iter
+  Vector.toListRev_iterFromIdx
+  Vector.toListRev_toIter
+  Vector.length_iterFromIdx
+  Vector.length_iter
